EDIT: Total code and Formal Verification

Exec.fst
@@ -1,5 +1,5 @@
 module Exec
- 
+
 (*
 Notaion: 
   - tos means top of stack (i.e., datastack[0])
@@ -40,6 +40,7 @@ let makeFrame virM code localplus global_names local_names =
     f_idCount = virM.idCount;
     f_usedIds = virM.usedIds
   } in
+
   let newVM: vm = {virM with callStack = frame::(virM.callStack)} in
   (newVM, frame)
 
@@ -48,11 +49,12 @@ let makeFrame virM code localplus global_names local_names =
   Ens:
 *)
 let call_function i globals dataStack id usedIds =
-  let args, newDataStack = List.splitAt i dataStack in
-  let localplus = List.Tot.Base.rev args in
-  let code, newDataStack = List.splitAt 1 newDataStack in
-  match List.hd code with
-  | CODEOBJECT co ->  
+  let args, newDataStack = splitAt i dataStack in
+  let localplus = rev args in
+  let code, restStack = splitAt 1 newDataStack in
+  match nth code 0 with
+  | None -> (undefinedBehavior "call_function_1")::dataStack
+  | Some (CODEOBJECT co) -> 
     let newFrame: frameObj = {
       dataStack = [];
       blockStack = [];
@@ -63,87 +65,139 @@ let call_function i globals dataStack id usedIds =
       f_locals = emptyMap;
       f_idCount = id;
       f_usedIds = usedIds
-    } in (FRAMEOBJECT newFrame)::dataStack
-  | _ -> All.failwith "CALL_FUNCTION: didn't call a function object"
+    } in (FRAMEOBJECT newFrame)::restStack
+  | _ -> (undefinedBehavior "call_function_2")::dataStack
 
 (*
    Req: length(datastack) >= 1
    Ens: res = datastack[1:]
 *)
-let pop_top datastack =  List.Tot.Base.tail datastack 
+
+let pop_top datastack = tail datastack
+
+let pop_top_rule (datastack: list pyObj {Cons? datastack})
+  : Lemma (requires length datastack >= 1)
+          (ensures  (length datastack)-1 = length (pop_top datastack))
+  = ()
 
 (*
    Req: length(datastack) >= 2
    Ens: res = tos1::tos::datastack[2:]
 *)
 let rot_two datastack = 
-  let tos = List.hd datastack in
-  let tos1 = List.nth datastack 1 in
-  let _, rest_stack = List.splitAt 2 datastack in
-  tos1::tos::rest_stack
+  let tos = hd datastack in
+  let tos1 = nth datastack 1 in
+  match tos1 with
+  | None -> (undefinedBehavior "rot_two")::datastack
+  | Some tos1 ->
+    let _, rest_stack = splitAt 2 datastack in
+    tos1::tos::rest_stack
 
+let rot_two_rule (datastack: list pyObj {Cons? datastack})
+  : Lemma (requires length datastack >= 2)
+          (ensures length (rot_two datastack) = length datastack 
+                 || length (rot_two datastack) = (length datastack)+1)
+  = ()
+  
 (*
    Req: length(datastack) >= 3
    Ens: res = tos1::tos2::tos::datastack[3:]
 *)
 let rot_three datastack = 
-  let tos = List.hd datastack in
-  let tos1 = List.nth datastack 1 in
-  let tos2 = List.nth datastack 2 in
-  let _, rest_stack = List.splitAt 3 datastack in
-  tos1::tos2::tos::rest_stack
+  let tos = hd datastack in
+  let tos1 = nth datastack 1 in
+  match tos1 with
+  | None -> (undefinedBehavior "rot_three_1")::datastack
+  | Some tos1 ->
+    let tos2 = nth datastack 2 in
+    (match tos2 with
+    | None -> (undefinedBehavior "rot_three_2")::datastack
+    | Some tos2 ->
+      let _, rest_stack = splitAt 3 datastack in
+      tos1::tos2::tos::rest_stack)
 
+let rot_three_rule (datastack: list pyObj {Cons? datastack})
+  : Lemma (requires length datastack >= 3)
+          (ensures length (rot_two datastack) = length datastack 
+                 || length (rot_two datastack) = (length datastack)+1)
+  = ()
+  
 (*
    Req: length(datastack) >= 4
    Ens: res = tos1::tos2::tos3::tos::datastack[4:]
 *)
 let rot_four datastack = 
-  let tos = List.hd datastack in
-  let tos1 = List.nth datastack 1 in
-  let tos2 = List.nth datastack 2 in
-  let tos3 = List.nth datastack 3 in
-  let _, rest_stack = List.splitAt 4 datastack in
-  tos1::tos2::tos3::tos::rest_stack
+  let tos = hd datastack in
+  let tos1 = nth datastack 1 in
+  match tos1 with
+  | None -> (undefinedBehavior "rot_four_1")::datastack
+  | Some tos1 ->
+    let tos2 = nth datastack 2 in
+    (match tos2 with
+    | None -> (undefinedBehavior "rot_four_2")::datastack
+    | Some tos2 ->
+      let tos3 = nth datastack 3 in
+      (match tos3 with
+      | None -> (undefinedBehavior "rot_four_3")::datastack
+      | Some tos3 ->
+        let _, rest_stack = splitAt 4 datastack in
+        tos1::tos2::tos3::tos::rest_stack))
+
+let rot_four_rule (datastack: list pyObj {Cons? datastack})
+  : Lemma (requires length datastack >= 4)
+          (ensures length (rot_two datastack) = length datastack 
+                 || length (rot_two datastack) = (length datastack)+1)
+  = ()
 
 (*
    Req: length(datastack) >= 1
    Ens: res = tos::datastack
 *)
-let dup_top datastack = 
-  let tos = List.hd datastack in
-  tos::datastack
+let dup_top datastack = (hd datastack)::datastack
 
+let dup_top_rule (datastack: list pyObj {Cons? datastack})
+  : Lemma (requires length datastack >= 1)
+          (ensures (length datastack)+1 = length (dup_top datastack))
+  = ()
+  
 (*
    Req: length(datastack) >= 2
    Ens: res = tos::tos1::datastack
 *)
 let dup_top_two datastack = 
-  let tos = List.hd datastack in
-  let tos1 = List.nth datastack 1 in
-  tos::tos1::datastack
+  let tos = hd datastack in
+  let tos1 = nth datastack 1 in
+  match tos1 with
+  | None -> (undefinedBehavior "dup_top")::datastack
+  | Some tos1 ->  tos::tos1::datastack
+
+let dup_top_two_rule (datastack: list pyObj {Cons? datastack})
+  : Lemma (requires length datastack >= 2)
+          (ensures (length datastack)+2 = length (dup_top_two datastack))
+  = ()
 
 (*
    Req: length(datastack) >= 1
-   Ens:
+   Ens: res = +tos::datastack[1:]
 *)
 let unary_positive datastack = 
-  let tos = List.hd datastack in
-  let newDataStack = List.tail datastack in
+  let tos = hd datastack in
+  let newDataStack = tail datastack in
   match tos with
   | PYTYP(obj) -> 
     (match (Map.sel (obj.methods) "__pos__") with
     | UNFUNBLT f -> PYTYP(builtinsToPyObj (f obj) )::newDataStack
     | ERR s -> PYTYP(createException "__pos__ is not defined" )::newDataStack
-    | _ -> (ERR "INTERPRTER UNDEFINED BEHAVIOR")::newDataStack)
-  | _ -> ERR("INTERPRTER UNDEFINED BEHAVIOR")::newDataStack
+    | _ -> (undefinedBehavior "unary_positive_1")::newDataStack)
+  | _ -> (undefinedBehavior "unary_positive_2")::newDataStack
   
 (*
    Req: length(datastack) >= 1
-   Ens:
+   Ens: res = -tos::datastack[1:]
 *)
 let unary_negative datastack  = 
-  let tos = List.hd datastack in
-  let newDataStack = List.tail datastack in
+  let tos = hd datastack in
+  let newDataStack = tail datastack in
   match tos with
   | PYTYP(obj) -> 
     (match (Map.sel (obj.methods) "__neg__") with
@@ -154,11 +208,11 @@ let unary_negative datastack  =
 
 (*
    Req: length(datastack) >= 1
-   Ens:
+   Ens: res = (not tos)::datastack[1:]
 *)
 let unary_not datastack  =
-  let tos = List.hd datastack in
-  let newDataStack = List.tail datastack in
+  let tos = hd datastack in
+  let newDataStack = tail datastack in
   match tos with
   | PYTYP(obj) ->
     let res = 
@@ -177,11 +231,11 @@ let unary_not datastack  =
 
 (*
    Req: length(datastack) >= 1
-   Ens:
+   Ens: res = iter(tos)::datastack[2:]
 *)
 let get_iter datastack  = 
-  let tos = List.hd datastack in
-  let newDataStack = List.tail datastack in
+  let tos = hd datastack in
+  let newDataStack = tail datastack in
   match tos with
   | PYTYP(obj) -> 
     (match (Map.sel (obj.methods) "__iter__") with
@@ -192,221 +246,253 @@ let get_iter datastack  =
 
 (*
   Req: length(datastack) >= 2
-  Ens: 
+  Ens: res = (tos1*tos)::datastack[2:]
 *)
-let binary_multiply (dataStack: list pyObj)  = 
-  let tos = List.hd dataStack in
-  let tos1 = List.nth dataStack 1 in
-  let (_, newDataStack) = List.splitAt 2 dataStack in 
-  match (tos, tos1) with
-  | PYTYP(obj1), PYTYP(obj2) -> 
-    (match (Map.sel (obj1.methods) "__mul__") with
-    | BINFUNBLT f -> PYTYP(builtinsToPyObj (f(obj1, obj2)) )::newDataStack
-    | ERR s -> PYTYP(createException "__mul__ is not defined" )::newDataStack
-    | _ -> (undefinedBehavior "binary_multiply_1")::newDataStack)
-  | _, _ -> (undefinedBehavior "binary_multiply_2")::newDataStack
+let binary_multiply dataStack  = 
+  let tos = hd dataStack in
+  let tos1 = nth dataStack 1 in
+  match tos1 with
+  | None -> (undefinedBehavior "binary_multiply_1")::dataStack
+  | Some tos1 ->
+    let (_, newDataStack) = splitAt 2 dataStack in 
+    match (tos, tos1) with
+    | PYTYP(obj1), PYTYP(obj2) -> 
+      (match (Map.sel (obj1.methods) "__mul__") with
+      | BINFUNBLT f -> PYTYP(builtinsToPyObj (f(obj1, obj2)) )::newDataStack
+      | ERR s -> PYTYP(createException "__mul__ is not defined" )::newDataStack
+      | _ -> (undefinedBehavior "binary_multiply_2")::newDataStack)
+    | _, _ -> (undefinedBehavior "binary_multiply_3")::newDataStack
 
 (*
   Req: length(datastack) >= 2
-  Ens: 
+  Ens: res = (tos1//tos)::datastack[2:]
 *)
-let binary_floor_divide (dataStack: list pyObj)  = 
-  let tos = List.hd dataStack in
-  let tos1 = List.nth dataStack 1 in
-  let (_, newDataStack) = List.splitAt 2 dataStack in 
-  match (tos, tos1) with
-  | PYTYP(obj1), PYTYP(obj2) -> 
-    (match (Map.sel (obj1.methods) "__floordiv__") with
-    | BINFUNBLT f -> PYTYP(builtinsToPyObj (f(obj1, obj2)) )::newDataStack
-    | ERR s -> PYTYP(createException "__floordiv__ is not defined" )::newDataStack
-    | _ -> (undefinedBehavior "binary_floor_divide_1")::newDataStack)
-  | _, _ -> (undefinedBehavior "binary_floor_divide_2")::newDataStack
+let binary_floor_divide dataStack  = 
+  let tos = hd dataStack in
+  let tos1 = nth dataStack 1 in
+  match tos1 with
+  | None -> (undefinedBehavior "binary_floor_divide_1")::dataStack
+  | Some tos1 ->
+    let (_, newDataStack) = splitAt 2 dataStack in 
+    match (tos, tos1) with
+    | PYTYP(obj1), PYTYP(obj2) -> 
+      (match (Map.sel (obj1.methods) "__floordiv__") with
+      | BINFUNBLT f -> PYTYP(builtinsToPyObj (f(obj1, obj2)) )::newDataStack
+      | ERR s -> PYTYP(createException "__floordiv__ is not defined" )::newDataStack
+      | _ -> (undefinedBehavior "binary_floor_divide_2")::newDataStack)
+    | _, _ -> (undefinedBehavior "binary_floor_divide_3")::newDataStack
 
 (*
   Req: length(datastack) >= 2
-  Ens: 
+  Ens: res = (tos1%tos)::datastack[2:]
 *)
-let binary_modulo (dataStack: list pyObj)  = 
-  let tos = List.hd dataStack in
-  let tos1 = List.nth dataStack 1 in
-  let (_, newDataStack) = List.splitAt 2 dataStack in 
-  match (tos, tos1) with
-  | PYTYP(obj1), PYTYP(obj2) -> 
-    (match (Map.sel (obj1.methods) "__mod__") with
-    | BINFUNBLT f -> PYTYP(builtinsToPyObj (f(obj1, obj2)) )::newDataStack
-    | ERR s -> PYTYP(createException "__mod__ is not defined" )::newDataStack
-    | _ -> (undefinedBehavior "binary_modulo_1")::newDataStack)
-  | _, _ -> (undefinedBehavior "binary_modulo_2")::newDataStack
-
+let binary_modulo dataStack =
+  let tos = hd dataStack in
+  let tos1 = nth dataStack 1 in
+  match tos1 with
+  | None -> (undefinedBehavior "bianry_modulo_1")::dataStack
+  | Some tos1 ->
+    let (_, newDataStack) = splitAt 2 dataStack in 
+    match (tos, tos1) with
+    | PYTYP(obj1), PYTYP(obj2) -> 
+      (match (Map.sel (obj1.methods) "__mod__") with
+      | BINFUNBLT f -> PYTYP(builtinsToPyObj (f(obj1, obj2)) )::newDataStack
+      | ERR s -> PYTYP(createException "__mod__ is not defined" )::newDataStack
+      | _ -> (undefinedBehavior "binary_modulo_2")::newDataStack)
+    | _, _ -> (undefinedBehavior "binary_modulo_3")::newDataStack
 
 (*
   Req: length(datastack) >= 2
-  Ens: 
+  Ens: res =(tos1+tos)::datastack[2:]
 *)
-let binary_add (dataStack: list pyObj)  = 
-  let tos = List.hd dataStack in
-  let tos1 = List.nth dataStack 1 in
-  let (_, newDataStack) = List.splitAt 2 dataStack in 
-  match (tos, tos1) with
-  | PYTYP(obj1), PYTYP(obj2) -> 
-    (match (Map.sel (obj1.methods) "__add__") with
-    | BINFUNBLT f -> PYTYP(builtinsToPyObj (f(obj1, obj2)) )::newDataStack
-    | ERR s -> PYTYP(createException "__add__ is not defined" )::newDataStack
-    | _ -> (undefinedBehavior "binary_add_1")::newDataStack)
-  | _, _ -> (undefinedBehavior "binary_add_2")::newDataStack
-
+let binary_add dataStack = 
+  let tos = hd dataStack in
+  let tos1 = nth dataStack 1 in
+  match tos1 with
+  | None -> (undefinedBehavior "binary_add_1")::dataStack
+  | Some tos1 ->
+    let (_, newDataStack) = splitAt 2 dataStack in
+    match (tos, tos1) with
+    | PYTYP(obj1), PYTYP(obj2) -> 
+      (match (Map.sel (obj1.methods) "__add__") with
+      | BINFUNBLT f -> PYTYP(builtinsToPyObj (f(obj1, obj2)) )::newDataStack
+      | ERR s -> PYTYP(createException "__add__ is not defined" )::newDataStack
+      | _ -> (undefinedBehavior "binary_add_2")::newDataStack)
+    | _, _ -> (undefinedBehavior "binary_add_3")::newDataStack
 
 (*
   Req: length(datastack) >= 2
-  Ens: 
+  Ens: res = (tos1-tos)::datastack[2:]
 *)
-let binary_subtract (dataStack: list pyObj)  = 
-  let tos = List.hd dataStack in
-  let tos1 = List.nth dataStack 1 in
-  let (_, newDataStack) = List.splitAt 2 dataStack in 
-  match (tos, tos1) with
-  | PYTYP(obj1), PYTYP(obj2) -> 
-    (match (Map.sel (obj1.methods) "__sub__") with
-    | BINFUNBLT f -> PYTYP(builtinsToPyObj (f(obj1, obj2)) )::newDataStack
-    | ERR s -> PYTYP(createException "__sub__ is not defined" )::newDataStack
-    | _ -> (undefinedBehavior "binary_subtract_1")::newDataStack)
-  | _, _ -> (undefinedBehavior "binary_subtract_2")::newDataStack
-
+let binary_subtract dataStack = 
+  let tos = hd dataStack in
+  let tos1 = nth dataStack 1 in
+  match tos1 with
+  | None -> (undefinedBehavior "binary_subtract_1")::dataStack
+  | Some tos1 ->
+    let (_, newDataStack) = splitAt 2 dataStack in 
+    match (tos, tos1) with
+    | PYTYP(obj1), PYTYP(obj2) -> 
+      (match (Map.sel (obj1.methods) "__sub__") with
+      | BINFUNBLT f -> PYTYP(builtinsToPyObj (f(obj1, obj2)) )::newDataStack
+      | ERR s -> PYTYP(createException "__sub__ is not defined" )::newDataStack
+      | _ -> (undefinedBehavior "binary_subtract_2")::newDataStack)
+    | _, _ -> (undefinedBehavior "binary_subtract_3")::newDataStack
 
 (*
   Req: length(datastack) >= 2
-  Ens: 
+  Ens: res = tos1[tos]::datastack[2:]
 *)
-let binary_subscr (dataStack: list pyObj)  = 
-  let tos = List.hd dataStack in
-  let tos1 = List.nth dataStack 1 in
-  let (_, newDataStack) = List.splitAt 2 dataStack in 
-  match (tos1, tos) with
-  | PYTYP(obj1), PYTYP(obj2) -> 
-    (match (Map.sel (obj1.methods) "__subscr__") with
-    | BINFUNBLT f -> PYTYP(builtinsToPyObj (f(obj1, obj2)) )::newDataStack
-    | ERR s -> PYTYP(createException "__subscr__ is not defined" )::newDataStack
-    | _ -> (undefinedBehavior "binary_subscr_1")::newDataStack)
-  | _, _ -> (undefinedBehavior "binary_subscr_2")::newDataStack
-
+let binary_subscr dataStack = 
+  let tos = hd dataStack in
+  let tos1 = nth dataStack 1 in
+  match tos1 with
+  | None -> (undefinedBehavior "binary_subscr_1")::dataStack
+  | Some tos1 ->
+    let (_, newDataStack) = splitAt 2 dataStack in 
+    match (tos1, tos) with
+    | PYTYP(obj1), PYTYP(obj2) -> 
+      (match (Map.sel (obj1.methods) "__subscr__") with
+      | BINFUNBLT f -> PYTYP(builtinsToPyObj (f(obj1, obj2)) )::newDataStack
+      | ERR s -> PYTYP(createException "__subscr__ is not defined" )::newDataStack
+      | _ -> (undefinedBehavior "binary_subscr_2")::newDataStack)
+    | _, _ -> (undefinedBehavior "binary_subscr_3")::newDataStack
 
 (*
   Req: (length(datastack) >= i)
-  Ens:
+  Ens: res = (tos, ..., tosi)::datastack[i+1:]
 *)
 let build_tuple i dataStack  =
-  let elems, newDataStack  = List.splitAt i dataStack in
-    let newDataStack = PYTYP(createTuple(List.map pyObjToobj elems) )::newDataStack in
-  newDataStack
+  let elems, newDataStack  = splitAt i dataStack in
+  match unwrapPyObjList elems with
+  | None -> (undefinedBehavior "build_tuple")::dataStack
+  | Some l -> PYTYP(createTuple l)::newDataStack
 
 (*
   Req: (length(datastack) >= i)
-  Ens:
+  Ens: res = [tos, ..., tosi]::datastack[i+1:]
 *)
 let build_list i dataStack  =
-  let elems, newDataStack  = List.splitAt i dataStack in
-  let newDataStack = PYTYP(createList(List.map pyObjToobj elems) )::newDataStack in
-  newDataStack
-
-(*
-  Req: (length(datastack) >= 1+conut)
-  Ens:
-*)
-let build_map count dataStack  =
-  let elems, newDataStack  = List.splitAt (op_Multiply 2 count) dataStack in
-  let clsElems = List.map pyObjToobj elems in
-  let vkl = listToPairs clsElems in
-  let newDataStack = PYTYP(createDict vkl)::newDataStack in
-  newDataStack
+  let elems, newDataStack  = splitAt i dataStack in
+  match unwrapPyObjList elems with
+  | None -> (undefinedBehavior "build_list")::dataStack
+  | Some l -> PYTYP(createList l)::newDataStack
 
 (*
   Req: (length(datastack) >= 2*conut)
-  Ens:
+  Ens: res = {..., TOS3: TOS2, TOS1: TOS}::datastack[2*count+1:]
+*)
+let build_map count dataStack  =
+  let elems, newDataStack  = splitAt (op_Multiply 2 count) dataStack in
+  match unwrapPyObjList elems with
+  | None -> (undefinedBehavior "build_map_1")::dataStack
+  | Some clsElems ->
+    (match (length clsElems)%2 = 0 with
+    | false -> (undefinedBehavior "build_map_2")::dataStack
+    | true -> 
+      let vkl = listToPairs clsElems in
+      let newDataStack = PYTYP(createDict vkl)::newDataStack in
+      newDataStack)
+
+(*
+  Req: (length(datastack) >= conut+1)
+  Ens: res = DICT(tos, [tos1, .. tosi])::datastack[i+2:]
 *)
 let build_const_key_map count dataStack  =
-  let keysObj, newDataStack = List.splitAt 1 dataStack in
+  let keysObj, newDataStack = splitAt 1 dataStack in
   match keysObj with
   | [PYTYP obj] ->
     (match obj.value with
     | TUPLE keysCls ->
-      (let vals, newDataStack  = List.splitAt count newDataStack in
-       let valsCls = List.map pyObjToobj vals in
-       let vkl = List.zip valsCls keysCls in
-       let newDataStack = PYTYP(createDict vkl)::newDataStack in
-       newDataStack)
-    | _ -> (undefinedBehavior "build_const_key_map_1")::newDataStack)
-  | _ -> (undefinedBehavior "build_const_key_map_2")::newDataStack
+      (let vals, newDataStack  = splitAt count newDataStack in
+       (match unwrapPyObjList vals with
+       | None -> (undefinedBehavior "build_const_key_map_2")::newDataStack
+       | Some valsCls ->
+         (match length valsCls = length keysCls with
+         | false -> (undefinedBehavior "build_const_key_map")::dataStack
+         | true -> 
+           let vkl = totZip valsCls keysCls in
+           let newDataStack = PYTYP(createDict vkl)::newDataStack in
+           newDataStack)))
+    | _ -> (undefinedBehavior "build_const_key_map_2")::newDataStack)
+  | _ -> (undefinedBehavior "build_const_key_map_3")::newDataStack
   
 (*
-  Req:
-  Ens:
+  Req: length(datastack) >= 2
+  Ens: res = (op tos1 tos)::datastack[2:]
 *)
 let compare_op i dataStack  =
-  let tos = List.hd dataStack in
-  let tos1 = List.nth dataStack 1 in
-  let (_, newDataStack) = List.splitAt 2 dataStack in
-  let op =
-    match i with
-    | 0 -> "__lt__"
-    | 1 -> "__le__"
-    | 2 -> "__eq__"
-    | 3 -> "__ne__"
-    | 4 -> "__gt__"
-    | 5 -> "__ge__"
-    | 6 -> "__contains__" (* in *)
-    | 7 -> "__contains__" (* not in*)
-    | 8 -> "__is__"
-    | 9 -> "__nis__"
-    | _ -> "error" in
-  match op with
-  | "__eq__" ->
-    (match (tos1, tos) with
-    | PYTYP(obj1), PYTYP(obj2) -> 
-      (match (Map.sel (obj1.methods) op) with
-      | BINFUNBLT f -> 
-        (match f(obj1, obj2) with
-          | BOOL b -> PYTYP(createBool b )::newDataStack
-          | _ -> PYTYP(createBool (obj1.pid = obj2.pid) )::newDataStack)
-      | _ -> (undefinedBehavior "compare_op_eq_1")::newDataStack)
-    | _,_ -> (undefinedBehavior "compare_op_eq_2")::newDataStack)
-  | "__ne__" ->
-    (match (tos1, tos) with
-    | PYTYP(obj1), PYTYP(obj2) -> 
-      (match (Map.sel (obj1.methods) op) with
-      | BINFUNBLT f -> 
-        (match f(obj1, obj2) with
-          | BOOL b -> PYTYP(createBool b )::newDataStack
-          | _ -> PYTYP(createBool (obj1.pid <> obj2.pid) )::newDataStack)
-      | _ -> (undefinedBehavior "compare_op_ne_1")::newDataStack)
-    | _,_ -> (undefinedBehavior "compare_op_ne_2")::newDataStack)
-  | "__is__" ->
-    (match (tos1, tos) with
-    | PYTYP(obj1), PYTYP(obj2) -> PYTYP(createBool (obj1.pid = obj2.pid) )::newDataStack
-    | _ -> (undefinedBehavior "compare_op_is")::newDataStack)
-  | "__nis__" ->
-    (match (tos1, tos) with
-    | PYTYP(obj1), PYTYP(obj2) -> PYTYP(createBool (obj1.pid <> obj2.pid) )::newDataStack
-    | _ -> (undefinedBehavior "compare_op_nis")::newDataStack)
-  | "error" -> (undefinedBehavior "compare_op_error")::newDataStack
-  | _ ->
-    match (tos1, tos) with
-    | PYTYP(obj1), PYTYP(obj2) -> 
-      (match (Map.sel (obj1.methods) op) with
-      | BINFUNBLT f -> PYTYP(builtinsToPyObj (f(obj1, obj2)) )::newDataStack
-      | ERR s -> PYTYP(createException "__pos__ is not defined" )::newDataStack
-      | _ -> (undefinedBehavior "compare_op_1")::newDataStack)
-    | _, _ -> (undefinedBehavior "compare_op_2")::newDataStack
+  let tos = hd dataStack in
+  let tos1 = nth dataStack 1 in
+  match tos1 with
+  | None -> (undefinedBehavior "compare_op_3")::dataStack
+  | Some tos1 -> 
+    let (_, newDataStack) = splitAt 2 dataStack in
+    let op =
+      match i with
+      | 0 -> "__lt__"
+      | 1 -> "__le__"
+      | 2 -> "__eq__"
+      | 3 -> "__ne__"
+      | 4 -> "__gt__"
+      | 5 -> "__ge__"
+      | 6 -> "__contains__" (* in *)
+      | 7 -> "__contains__" (* not in*)
+      | 8 -> "__is__"
+      | 9 -> "__nis__"
+      | _ -> "error" in
+    match op with
+    | "__eq__" ->
+      (match (tos1, tos) with
+      | PYTYP(obj1), PYTYP(obj2) -> 
+        (match (Map.sel (obj1.methods) op) with
+        | BINFUNBLT f -> 
+          (match f(obj1, obj2) with
+            | BOOL b -> PYTYP(createBool b )::newDataStack
+            | _ -> PYTYP(createBool (obj1.pid = obj2.pid) )::newDataStack)
+        | _ -> (undefinedBehavior "compare_op_eq_1")::newDataStack)
+      | _,_ -> (undefinedBehavior "compare_op_eq_2")::newDataStack)
+    | "__ne__" ->
+      (match (tos1, tos) with
+      | PYTYP(obj1), PYTYP(obj2) -> 
+        (match (Map.sel (obj1.methods) op) with
+        | BINFUNBLT f -> 
+          (match f(obj1, obj2) with
+            | BOOL b -> PYTYP(createBool b )::newDataStack
+            | _ -> PYTYP(createBool (obj1.pid <> obj2.pid) )::newDataStack)
+        | _ -> (undefinedBehavior "compare_op_ne_1")::newDataStack)
+      | _,_ -> (undefinedBehavior "compare_op_ne_2")::newDataStack)
+    | "__is__" ->
+      (match (tos1, tos) with
+      | PYTYP(obj1), PYTYP(obj2) -> PYTYP(createBool (obj1.pid = obj2.pid) )::newDataStack
+      | _ -> (undefinedBehavior "compare_op_is")::newDataStack)
+    | "__nis__" ->
+      (match (tos1, tos) with
+      | PYTYP(obj1), PYTYP(obj2) -> PYTYP(createBool (obj1.pid <> obj2.pid) )::newDataStack
+      | _ -> (undefinedBehavior "compare_op_nis")::newDataStack)
+    | "error" -> (undefinedBehavior "compare_op_error")::newDataStack
+    | _ ->
+      match (tos1, tos) with
+      | PYTYP(obj1), PYTYP(obj2) -> 
+        (match (Map.sel (obj1.methods) op) with
+        | BINFUNBLT f -> PYTYP(builtinsToPyObj (f(obj1, obj2)) )::newDataStack
+        | ERR s -> PYTYP(createException "__pos__ is not defined" )::newDataStack
+        | _ -> (undefinedBehavior "compare_op_2")::newDataStack)
+      | _, _ -> (undefinedBehavior "compare_op_3")::newDataStack
 
 (*
-  Req:
-  Ens:
+  Req: (length names) >= i && (length datastack) > 1 
+  Ens: res = (f_locals with f_locals[name] = tos, datastack[1:])
 *)
 let store_name i names f_locals dataStack = 
-  let name = List.nth names i in
-  let tos = List.hd dataStack in
-  let _, newDataStack = List.splitAt 1 dataStack in 
-  let newLocals = Map.upd f_locals name tos in
-  (newLocals, newDataStack)
+  let tos = hd dataStack in
+  let name = nth names i in
+  match name with
+  | None -> (f_locals, (undefinedBehavior "store_name")::dataStack)
+  | Some name -> 
+    let _, newDataStack = splitAt 1 dataStack in 
+    let newLocals = Map.upd f_locals name tos in
+    (newLocals, newDataStack)
   
   
 (*
@@ -414,30 +500,38 @@ let store_name i names f_locals dataStack =
   Ens: res = consts[i]::datastack
 *)
 let load_const i consts dataStack =
-  let elem = List.nth consts i in
-  let newDataStack = elem::dataStack in
-  newDataStack
+  let elem = nth consts i in
+  match elem with
+  | None -> (undefinedBehavior "load_constant")::dataStack
+  | Some elem ->
+    let newDataStack = elem::dataStack in
+    newDataStack
 
 (*
-  Req:
-  Ens:
+  Req: (length names) > i
+  Ens: res = f_locals[names[i]]::datastack  ||
+       res = f_globals[names[i]]::datastack ||
+       res = exception::datastack
 *)
 let load_name i names f_locals f_globals dataStack  =
-  let name = List.nth names i in
-  match Map.contains f_locals name with
-   | true -> (Map.sel f_locals name)::dataStack 
-   | false ->
-     (match Map.contains f_globals name with
-      | true -> (Map.sel f_globals name)::dataStack
-      | false -> PYTYP(createException ("name: " ^ name ^ "is not defined") )::dataStack)
+  let name = nth names i in
+  match name with
+  | None -> (undefinedBehavior "load_name")::dataStack
+  | Some name ->
+    (match Map.contains f_locals name with
+    | true -> (Map.sel f_locals name)::dataStack 
+    | false ->
+      (match Map.contains f_globals name with
+       | true -> (Map.sel f_globals name)::dataStack
+       | false -> PYTYP(createException ("name: " ^ name ^ "is not defined"))::dataStack))
 
 (*
-  Req:
+  Req: 
   Ens:
 *)
 let pop_jump_if_true i pc dataStack  =
-  let tos = List.hd dataStack in
-  let newDataStack = List.tail dataStack in
+  let tos = hd dataStack in
+  let newDataStack = tail dataStack in
   match tos with
   | PYTYP(obj) ->
     (match obj.value with
@@ -450,8 +544,8 @@ let pop_jump_if_true i pc dataStack  =
   Ens:
 *)
 let pop_jump_if_false i pc dataStack  =
-  let tos = List.hd dataStack in
-  let newDataStack = List.tail dataStack in
+  let tos = hd dataStack in
+  let newDataStack = tail dataStack in
   match tos with
   | PYTYP(obj) ->
     (match obj.value with
@@ -464,8 +558,8 @@ let pop_jump_if_false i pc dataStack  =
   Ens:
 *)
 let jump_if_true_or_pop i pc dataStack  =
-  let tos = List.hd dataStack in
-  let newDataStack = List.tail dataStack in
+  let tos = hd dataStack in
+  let newDataStack = tail dataStack in
   match tos with
   | PYTYP(obj) ->
     (match obj.value with
@@ -478,8 +572,8 @@ let jump_if_true_or_pop i pc dataStack  =
   Ens:
 *)
 let jump_if_false_or_pop i pc dataStack  =
-  let tos = List.hd dataStack in
-  let newDataStack = List.tail dataStack in
+  let tos = hd dataStack in
+  let newDataStack = tail dataStack in
   match tos with
   | PYTYP(obj) ->
     (match obj.value with
@@ -487,14 +581,13 @@ let jump_if_false_or_pop i pc dataStack  =
     | _ -> (pc, PYTYP(createException "ERR: argument is not a Bool" )::newDataStack))
   | _ -> (pc, (undefinedBehavior "jump_if_false_or_pop")::newDataStack)
 
-
 (*
    Req:
    Ens:
 *)
 let for_iter i pc dataStack  =
-  let tos = List.hd dataStack in
-  let newDataStack = List.tail dataStack in
+  let tos = hd dataStack in
+  let newDataStack = tail dataStack in
    match tos with
   | PYTYP(obj) -> 
     (match (Map.sel (obj.methods) "__next__") with
@@ -512,71 +605,80 @@ let for_iter i pc dataStack  =
   Ens:
 *)
 let load_global i names f_globals dataStack  =
-  let name = List.nth names i in
-  match Map.contains f_globals name with
-   | true -> (Map.sel f_globals name)::dataStack
-   | false -> PYTYP(createException ("name: " ^ name ^ "is not defined") )::dataStack
+  let name = nth names i in
+  match name with
+  | None -> (undefinedBehavior "load_global")::dataStack
+  | Some name ->
+    match Map.contains f_globals name with
+    | true -> (Map.sel f_globals name)::dataStack
+    | false -> PYTYP(createException ("name: " ^ name ^ "is not defined") )::dataStack
 
 (*
-  Req: (length(localplus) > i) && (length(datastack) >= 1)
+  Req: (length(localplus) > i)
   Ens: res = localplus[i]::dataStack
 *)
 let load_fast i localPlus dataStack =
-  let elem = List.nth localPlus i in
-  let newDataStack = elem::dataStack in
-  newDataStack
+  let elem = nth localPlus i in
+  match elem with
+  | None -> (undefinedBehavior "load_fast")::dataStack
+  | Some elem ->
+    let newDataStack = elem::dataStack in
+    newDataStack
 
 (*
-  Req: i >= (length(f_localplus)) && (length(datastack) >= 1)
+  Req: (length f_localplus) >= i 
   Ens: res = (localplus where localplus[i] = tos, datastack[1:])
 *)
 let store_fast i localplus dataStack =
-  let tos = List.hd dataStack in
-  let newDataStack = List.tail dataStack in
-    match (List.Tot.Base.length localplus) > i with
+  let tos = hd dataStack in
+  let newDataStack = tail dataStack in
+    match (length localplus) > i with
     | true ->
-      (let newLocalPlus = List.mapi (fun k x -> if k = i then tos else x) localplus in
-        (newLocalPlus, newDataStack))
+      let newLocalPlus = mapi (fun k x -> if k = i then tos else x) localplus in
+      (newLocalPlus, newDataStack)
     | false ->
-      (match (List.Tot.Base.length localplus) = i with
-       | true ->
-         (let newLocalPlus = List.append localplus [tos] in
-           (newLocalPlus, newDataStack)) 
-       | false -> (localplus, (ERR "STORE_FAST: storing out of index")::newDataStack))
+      let newLocalPlus = append localplus [tos] in
+      (newLocalPlus, newDataStack) 
 
 (*
   Req:
   Ens:
 *)
 let make_function flags globs dataStack =
-  let qualname = List.hd dataStack in
-  let codeobj = List.nth dataStack 1 in
-  let (_, newDataStack) = List.splitAt 2 dataStack in
-  let func = createFunction ({
-    func_Code = codeobj;
-    func_globals = globs;
-    func_name = qualname;
-    func_closure =
-      if flags = 8 then
-      (match List.hd newDataStack with
-       | PYTYP(obj) ->
-         (match obj.value with
-           | TUPLE(t) -> PYTYP(createTuple t)
-           | _ -> undefinedBehavior "make_function_func_closure_1")
-       | _ -> undefinedBehavior "make_function_func_closure_2") else PYTYP(createNone());
-   
-    func_defaults =
-      if flags = 1 then
-      (match  List.hd newDataStack with
-      | PYTYP(obj) ->
-         (match obj.value with
-           | TUPLE(t) -> PYTYP(createTuple t)
-           | _ -> undefinedBehavior "make_function_func_defaults_1")
-       | _ -> undefinedBehavior "make_function_func_defaults_2") else PYTYP(createNone());
-  }) in
-    (match flags with
-     | 0 -> PYTYP(func)::newDataStack
-     | _ -> PYTYP(func)::(List.tail newDataStack))
+  let qualname = hd dataStack in
+  let codeobj = nth dataStack 1 in
+  match codeobj with
+  | None -> (undefinedBehavior "make_function_1")::dataStack
+  | Some codeobj ->
+    let (_, newDataStack) = splitAt 2 dataStack in
+    (match newDataStack with
+    | [] -> (undefinedBehavior "make_function_2")::dataStack
+    | _ ->
+      let func = createFunction ({
+      func_Code = codeobj;
+      func_globals = globs;
+      func_name = qualname;
+      func_closure =
+        if flags = 8 then
+        (match hd newDataStack with
+         | PYTYP(obj) ->
+           (match obj.value with
+             | TUPLE(t) -> PYTYP(createTuple t)
+             | _ -> undefinedBehavior "make_function_func_closure_1")
+         | _ -> undefinedBehavior "make_function_func_closure_2") else PYTYP(createNone());
+
+      func_defaults =
+        if flags = 1 then
+        (match  hd newDataStack with
+        | PYTYP(obj) ->
+           (match obj.value with
+             | TUPLE(t) -> PYTYP(createTuple t)
+             | _ -> undefinedBehavior "make_function_func_defaults_1")
+         | _ -> undefinedBehavior "make_function_func_defaults_2") else PYTYP(createNone());
+    }) in
+      (match flags with
+       | 0 -> PYTYP(func)::newDataStack
+       | _ -> PYTYP(func)::(tail newDataStack)))
 
 (*
    Req: len(frame.fcode.bytecode) >= 1
@@ -589,119 +691,332 @@ let rec execBytecode frame  =
     let CODE(bc) = frame.fCode.co_code in
     match List.nth bc (frame.pc) with
     | RETURN_VALUE -> frame
-    | CALL_FUNCTION i -> 
-      let newDataStack = call_function i frame.f_globals frame.dataStack frame.f_idCount frame.f_usedIds in
-        ({frame with dataStack = newDataStack})
+    
+    | CALL_FUNCTION i ->
+      (match length frame.dataStack > i with
+      | false ->
+        let newDataStack = [undefinedBehavior "CALL_FUNCTION"] in
+          ({frame with dataStack = newDataStack})
+      | true ->
+        let newDataStack = call_function i frame.f_globals frame.dataStack
+                         frame.f_idCount frame.f_usedIds in
+        ({frame with dataStack = newDataStack}))
+    
     | NOP -> execBytecode ({frame with pc = frame.pc+1})
+    
     | POP_TOP ->
       (match frame.dataStack with
       | [] ->
-        let newDataStack = [undefinedBehavior "pop_top"] in
+        let newDataStack = [undefinedBehavior "POP_TOP"] in
           execBytecode ({frame with dataStack = newDataStack; pc = frame.pc+1})
       | _ ->
         let newDataStack = pop_top frame.dataStack in
           execBytecode ({frame with dataStack = newDataStack; pc = frame.pc+1}))
+    
     | ROT_TWO ->
-      let newDataStack = rot_two frame.dataStack in
-        execBytecode ({frame with dataStack = newDataStack; pc = frame.pc+1})
+      (match (length frame.dataStack) >= 2 with
+      | false ->
+        let newDataStack = [undefinedBehavior "ROT_TWO"] in
+          execBytecode ({frame with dataStack = newDataStack; pc = frame.pc+1})
+      | true ->
+        let newDataStack = rot_two frame.dataStack in
+          execBytecode ({frame with dataStack = newDataStack; pc = frame.pc+1}))
+    
     | ROT_THREE ->
-      let newDataStack = rot_three frame.dataStack in
-        execBytecode ({frame with dataStack = newDataStack; pc = frame.pc+1})
+      (match length frame.dataStack >= 3 with
+      | false ->
+        let newDataStack = [undefinedBehavior "ROT_THREE"] in
+          execBytecode ({frame with dataStack = newDataStack; pc = frame.pc+1})
+      | true ->
+        let newDataStack = rot_three frame.dataStack in
+          execBytecode ({frame with dataStack = newDataStack; pc = frame.pc+1}))
+    
     | ROT_FOUR ->
-      let newDataStack = rot_four frame.dataStack in
-        execBytecode ({frame with dataStack = newDataStack; pc = frame.pc+1})
+      (match length frame.dataStack >= 4 with
+      | false ->
+        let newDataStack = [undefinedBehavior "ROT_FOUR"] in
+          execBytecode ({frame with dataStack = newDataStack; pc = frame.pc+1})
+      | true ->
+        let newDataStack = rot_four frame.dataStack in
+          execBytecode ({frame with dataStack = newDataStack; pc = frame.pc+1}))
+    
     | DUP_TOP ->
-      let newDataStack = dup_top frame.dataStack in
-        execBytecode ({frame with dataStack = newDataStack; pc = frame.pc+1})
+      (match frame.dataStack with
+      | [] ->
+        let newDataStack = [undefinedBehavior "DUP_TOP"] in
+          execBytecode ({frame with dataStack = newDataStack; pc = frame.pc+1})
+      | _ ->
+        let newDataStack = dup_top frame.dataStack in
+          execBytecode ({frame with dataStack = newDataStack; pc = frame.pc+1}))
+    
     | DUP_TOP_TWO ->
-      let newDataStack = dup_top_two frame.dataStack in
-        execBytecode ({frame with dataStack = newDataStack; pc = frame.pc+1})
+      (match length frame.dataStack >= 2 with
+      | false ->
+        let newDataStack = [undefinedBehavior "DUP_TOP_TWO"] in
+          execBytecode ({frame with dataStack = newDataStack; pc = frame.pc+1})
+      | true ->
+        let newDataStack = dup_top_two frame.dataStack in
+          execBytecode ({frame with dataStack = newDataStack; pc = frame.pc+1}))
+    
     | UNARY_POSITIVE ->
-      let newDataStack = unary_positive frame.dataStack in
-        execBytecode ({frame with dataStack = newDataStack; pc = frame.pc+1})
+      (match frame.dataStack with
+      | [] -> 
+        let newDataStack = [undefinedBehavior "UNARY_POSITIVE"] in
+          execBytecode ({frame with dataStack = newDataStack; pc = frame.pc+1})
+      | _ ->
+        let newDataStack = unary_positive frame.dataStack in
+          execBytecode ({frame with dataStack = newDataStack; pc = frame.pc+1}))
+    
     | UNARY_NEGATIVE ->
-      let newDataStack = unary_negative frame.dataStack in
-        execBytecode ({frame with dataStack = newDataStack; pc = frame.pc+1})
+      (match frame.dataStack with
+      | [] ->
+        let newDataStack = [undefinedBehavior "UNARY_NEGATIVE"] in
+          execBytecode ({frame with dataStack = newDataStack; pc = frame.pc+1})
+      | _ ->
+        let newDataStack = unary_negative frame.dataStack in
+          execBytecode ({frame with dataStack = newDataStack; pc = frame.pc+1}))
+    
     | UNARY_NOT ->
-      let newDataStack = unary_not frame.dataStack in
-        execBytecode ({frame with dataStack = newDataStack; pc = frame.pc+1})
+      (match frame.dataStack with
+      | [] ->
+        let newDataStack = [undefinedBehavior "UNARY_NOT"] in
+          execBytecode ({frame with dataStack = newDataStack; pc = frame.pc+1})
+      | _ ->
+        let newDataStack = unary_not frame.dataStack in
+          execBytecode ({frame with dataStack = newDataStack; pc = frame.pc+1}))
+    
     | GET_ITER ->
-      let newDataStack = get_iter frame.dataStack in
-        execBytecode ({frame with dataStack = newDataStack; pc = frame.pc+1})
-    | BINARY_MULTIPLY -> 
-      let newDataStack = binary_multiply (frame.dataStack) in
-        execBytecode ({frame with dataStack = newDataStack; pc = frame.pc+1})
-    | BINARY_FLOOR_DIVIDE -> 
-      let newDataStack = binary_floor_divide (frame.dataStack) in
-        execBytecode ({frame with dataStack = newDataStack; pc = frame.pc+1})    
-    | BINARY_MODULO -> 
-      let newDataStack = binary_modulo (frame.dataStack) in
-        execBytecode ({frame with dataStack = newDataStack; pc = frame.pc+1})
-    | BINARY_ADD -> 
-      let newDataStack = binary_add (frame.dataStack) in
-        execBytecode ({frame with dataStack = newDataStack; pc = frame.pc+1})    
-    | BINARY_SUBTRACT -> 
-      let newDataStack = binary_subtract (frame.dataStack) in
-        execBytecode ({frame with dataStack = newDataStack; pc = frame.pc+1}) 
-    | BINARY_SUBSCR -> 
-      let newDataStack = binary_subtract (frame.dataStack) in
-        execBytecode ({frame with dataStack = newDataStack; pc = frame.pc+1}) 
+      (match frame.dataStack with
+      | [] ->
+        let newDataStack = [undefinedBehavior "GET_ITER"] in
+          execBytecode ({frame with dataStack = newDataStack; pc = frame.pc+1})
+      | _ ->
+        let newDataStack = get_iter frame.dataStack in
+          execBytecode ({frame with dataStack = newDataStack; pc = frame.pc+1}))
+    
+    | BINARY_MULTIPLY ->
+      (match length frame.dataStack >= 2 with
+      | false ->
+        let newDataStack = [undefinedBehavior "BINARY_MULTIPLY"] in
+          execBytecode ({frame with dataStack = newDataStack; pc = frame.pc+1})
+      | true ->
+        let newDataStack = binary_multiply (frame.dataStack) in
+          execBytecode ({frame with dataStack = newDataStack; pc = frame.pc+1}))
+    
+    | BINARY_FLOOR_DIVIDE ->
+      (match length frame.dataStack >= 2 with
+      | false ->
+        let newDataStack = [undefinedBehavior "BINARY_FLOOR_DIVIDE"] in
+          execBytecode ({frame with dataStack = newDataStack; pc = frame.pc+1})
+      | true ->
+        let newDataStack = binary_floor_divide (frame.dataStack) in
+          execBytecode ({frame with dataStack = newDataStack; pc = frame.pc+1}))
+    
+    | BINARY_MODULO ->
+      (match length frame.dataStack >= 2 with
+      | false ->
+        let newDataStack = [undefinedBehavior "BINARY_MODULO"] in
+          execBytecode ({frame with dataStack = newDataStack; pc = frame.pc+1})
+      | true ->
+        let newDataStack = binary_modulo (frame.dataStack) in
+          execBytecode ({frame with dataStack = newDataStack; pc = frame.pc+1}))
+    
+    | BINARY_ADD ->
+      (match length frame.dataStack >= 2 with
+      | false ->
+        let newDataStack = [undefinedBehavior "BINARY_ADD"] in
+          execBytecode ({frame with dataStack = newDataStack; pc = frame.pc+1})
+      | true ->
+        let newDataStack = binary_add (frame.dataStack) in
+          execBytecode ({frame with dataStack = newDataStack; pc = frame.pc+1}))
+    
+    | BINARY_SUBTRACT ->
+      (match length frame.dataStack >= 2 with
+      | false ->
+        let newDataStack = [undefinedBehavior "BINARY_SUBTRACT"] in
+          execBytecode ({frame with dataStack = newDataStack; pc = frame.pc+1})
+      | true ->
+        let newDataStack = binary_subtract (frame.dataStack) in
+          execBytecode ({frame with dataStack = newDataStack; pc = frame.pc+1}))
+    
+    | BINARY_SUBSCR ->
+      (match length frame.dataStack >= 2 with
+      | false ->
+        let newDataStack = [undefinedBehavior "BINARY_SUBSCR"] in
+          execBytecode ({frame with dataStack = newDataStack; pc = frame.pc+1})
+      | true ->
+        let newDataStack = binary_subtract (frame.dataStack) in
+          execBytecode ({frame with dataStack = newDataStack; pc = frame.pc+1})) 
+    
     | LOAD_CONST(i) ->
-      let newDataStack = load_const i (frame.fCode.co_consts) (frame.dataStack) in
-        execBytecode ({frame with dataStack = newDataStack; pc = frame.pc+1})
+      (match length frame.fCode.co_consts > i with
+      | fasle -> 
+        let newDataStack = [undefinedBehavior "LOAD_CONST"] in
+          execBytecode ({frame with dataStack = newDataStack; pc = frame.pc+1})
+      | true ->
+        let newDataStack = load_const i (frame.fCode.co_consts)
+                           (frame.dataStack) in
+          execBytecode ({frame with dataStack = newDataStack; pc = frame.pc+1}))
+    
     | LOAD_NAME(i) ->
-      let newDataStack = load_name i (frame.fCode.co_names) (frame.f_locals) (frame.f_globals) (frame.dataStack) in
-        execBytecode ({frame with dataStack = newDataStack; pc = frame.pc+1})
+      (match length frame.fCode.co_names > i with
+      | false -> 
+        let newDataStack = [undefinedBehavior "LOAD_NAME"] in
+          execBytecode ({frame with dataStack = newDataStack; pc = frame.pc+1})
+      | true -> 
+        let newDataStack = load_name i (frame.fCode.co_names) (frame.f_locals)
+                           (frame.f_globals) (frame.dataStack) in
+          execBytecode ({frame with dataStack = newDataStack; pc = frame.pc+1}))
+    
     | BUILD_TUPLE(i) ->
-      let newDataStack = build_tuple i (frame.dataStack) in
-        execBytecode ({frame with dataStack = newDataStack; pc = frame.pc+1})
+      (match length frame.dataStack >= i with
+      | false ->
+        let newDataStack = [undefinedBehavior "BUILD_TUPLE"] in
+          execBytecode ({frame with dataStack = newDataStack; pc = frame.pc+1})
+      | true -> 
+        let newDataStack = build_tuple i (frame.dataStack) in
+          execBytecode ({frame with dataStack = newDataStack; pc = frame.pc+1}))
+     
     | STORE_NAME(i) ->
-      let newLocals, newDataStack = store_name i (frame.fCode.co_names) (frame.f_locals) (frame.dataStack) in
-        execBytecode ({frame with dataStack = newDataStack; pc = frame.pc+1; f_locals = newLocals})
+      (match length frame.fCode.co_names > i && length frame.dataStack >= 1 with
+      | false ->
+        let newDataStack = [undefinedBehavior "STORE_NAME"] in
+          execBytecode ({frame with dataStack = newDataStack; pc = frame.pc+1})
+      | true ->
+        let newLocals, newDataStack = store_name i (frame.fCode.co_names)
+                                      (frame.f_locals) (frame.dataStack) in
+            execBytecode ({frame with dataStack = newDataStack; 
+                                      pc = frame.pc+1;
+                                      f_locals = newLocals}))
+
     |  BUILD_LIST(i) ->
-      let newDataStack = build_list i (frame.dataStack) in
-        execBytecode ({frame with dataStack = newDataStack; pc = frame.pc+1})
+      (match length frame.dataStack >= i with
+      | false ->
+        let newDataStack = [undefinedBehavior "BUILD_LIST"] in
+          execBytecode ({frame with dataStack = newDataStack; pc = frame.pc+1})
+      | true ->
+        let newDataStack = build_list i (frame.dataStack) in
+          execBytecode ({frame with dataStack = newDataStack; pc = frame.pc+1}))
+    
     | BUILD_MAP(i) ->
-      let newDataStack = build_map i (frame.dataStack) in
-        execBytecode ({frame with dataStack = newDataStack; pc = frame.pc+1})
+      (match length frame.dataStack >= (op_Multiply 2 i) with
+      | false ->
+        let newDataStack = [undefinedBehavior "BUILD_MAP"] in
+          execBytecode ({frame with dataStack = newDataStack; pc = frame.pc+1})
+      | true -> 
+        let newDataStack = build_map i (frame.dataStack) in
+          execBytecode ({frame with dataStack = newDataStack; pc = frame.pc+1}))
+    
     | BUILD_CONST_KEY_MAP(i) ->
-      let newDataStack = build_const_key_map i (frame.dataStack) in
-        execBytecode ({frame with dataStack = newDataStack; pc = frame.pc+1})
+      (match length frame.dataStack >= i+1 with
+      | false ->
+        let newDataStack = [undefinedBehavior "BUILD_CONST_KEY_MAP"] in
+          execBytecode ({frame with dataStack = newDataStack; pc = frame.pc+1})
+      | true -> 
+        let newDataStack = build_const_key_map i (frame.dataStack) in
+          execBytecode ({frame with dataStack = newDataStack; pc = frame.pc+1}))
+        
     | JUMP_FORWARD(i) -> execBytecode ({frame with pc = frame.pc + (i/2) + 1})
+    
     | POP_JUMP_IF_TRUE(i) ->
-      let newPc, newDataStack = pop_jump_if_true i (frame.pc) (frame.dataStack) in
-      let newPc = if frame.pc=newPc then newPc+1 else newPc in
-        execBytecode ({frame with dataStack = newDataStack; pc = newPc})
+      (match frame.dataStack with
+      | [] ->
+        let newDataStack = [undefinedBehavior "POP_JUMP_IF_TRUE"] in
+          execBytecode ({frame with dataStack = newDataStack; pc = frame.pc+1})
+      | _ ->
+        let newPc, newDataStack = pop_jump_if_true i (frame.pc)
+                                                     (frame.dataStack) in
+        let newPc = if frame.pc=newPc then newPc+1 else newPc in
+          execBytecode ({frame with dataStack = newDataStack; pc = newPc}))
+    
     | POP_JUMP_IF_FALSE(i) ->
-      let newPc, newDataStack = pop_jump_if_false i (frame.pc) (frame.dataStack) in
-      let newPc = if frame.pc=newPc then newPc+1 else newPc in
-        execBytecode ({frame with dataStack = newDataStack; pc = newPc})
+      (match frame.dataStack with
+      | [] ->
+        let newDataStack = [undefinedBehavior "POP_JUMP_IF_FALSE"] in
+          execBytecode ({frame with dataStack = newDataStack; pc = frame.pc+1})
+      | _ ->
+        let newPc, newDataStack = pop_jump_if_false i (frame.pc) 
+                                                      (frame.dataStack) in
+        let newPc = if frame.pc=newPc then newPc+1 else newPc in
+          execBytecode ({frame with dataStack = newDataStack; pc = newPc}))
+    
     | JUMP_IF_TRUE_OR_POP(i) ->
-      let newPc, newDataStack = jump_if_true_or_pop i (frame.pc) (frame.dataStack) in
-      let newPc = if frame.pc=newPc then newPc+1 else newPc in
-        execBytecode ({frame with dataStack = newDataStack; pc = newPc})
+      (match frame.dataStack with
+      | [] ->
+        let newDataStack = [undefinedBehavior "JUMP_IF_TRUE_OR_POP"] in
+          execBytecode ({frame with dataStack = newDataStack; pc = frame.pc+1})
+      | _ ->
+        let newPc, newDataStack = jump_if_true_or_pop i (frame.pc)
+                                                        (frame.dataStack) in
+        let newPc = if frame.pc=newPc then newPc+1 else newPc in
+          execBytecode ({frame with dataStack = newDataStack; pc = newPc}))
+    
     | JUMP_IF_FALSE_OR_POP(i) ->
-      let newPc, newDataStack = jump_if_false_or_pop i (frame.pc) (frame.dataStack) in
-      let newPc = if frame.pc=newPc then newPc+1 else newPc in
-        execBytecode ({frame with dataStack = newDataStack; pc = newPc})
+      (match frame.dataStack with
+      | [] ->
+        let newDataStack = [undefinedBehavior "JUMP_IF_FALSE_OR_POP"] in
+          execBytecode ({frame with dataStack = newDataStack; pc = frame.pc+1})
+      | _ ->
+        let newPc, newDataStack = jump_if_false_or_pop i (frame.pc) 
+                                                         (frame.dataStack) in
+        let newPc = if frame.pc=newPc then newPc+1 else newPc in
+          execBytecode ({frame with dataStack = newDataStack; pc = newPc}))
+    
     | FOR_ITER(i) ->
-      let newPc, newDataStack = for_iter i (frame.pc) (frame.dataStack) in
-      let newPc = if frame.pc=newPc then newPc+1 else newPc in
-        execBytecode ({frame with dataStack = newDataStack; pc = newPc})
+      (match frame.dataStack with
+      | [] -> 
+        let newDataStack = [undefinedBehavior "FOR_ITER"] in
+          execBytecode ({frame with dataStack = newDataStack; pc = frame.pc+1})
+      | _ ->
+        let newPc, newDataStack = for_iter i (frame.pc) (frame.dataStack) in
+        let newPc = if frame.pc=newPc then newPc+1 else newPc in
+          execBytecode ({frame with dataStack = newDataStack; pc = newPc}))
+    
     | JUMP_ABSOLUTE(i) -> execBytecode ({frame with pc = i/2})
+    
     | LOAD_GLOBAL(i) ->
-      let newDataStack = load_global i (frame.fCode.co_names) (frame.f_globals) (frame.dataStack) in
-        execBytecode ({frame with dataStack = newDataStack; pc = frame.pc+1})
+      (match length frame.fCode.co_names > i with
+      | false -> 
+        let newDataStack = [undefinedBehavior "LOAD_GLOBAL"] in
+          execBytecode ({frame with dataStack = newDataStack; pc = frame.pc+1})
+      | true ->
+        let newDataStack = load_global i (frame.fCode.co_names) (frame.f_globals) 
+                                         (frame.dataStack) in
+          execBytecode ({frame with dataStack = newDataStack; pc = frame.pc+1}))
+    
     | LOAD_FAST(i) ->
-      let newDataStack = load_fast i (frame.f_localplus) (frame.dataStack) in
-        execBytecode ({frame with dataStack = newDataStack; pc = frame.pc+1})   
+      (match length frame.f_localplus > i with
+      | false ->  
+        let newDataStack = [undefinedBehavior "LOAD_FAST"] in
+          execBytecode ({frame with dataStack = newDataStack; pc = frame.pc+1})
+      | true ->
+        let newDataStack = load_fast i (frame.f_localplus) (frame.dataStack) in
+          execBytecode ({frame with dataStack = newDataStack; pc = frame.pc+1}))
+    
     | STORE_FAST(i) ->
-      let newLocalPlus, newDataStack = store_fast i (frame.f_localplus) (frame.dataStack) in
-        execBytecode ({frame with dataStack = newDataStack; pc = frame.pc+1; f_localplus = newLocalPlus})
+      (match length frame.f_localplus >= i && length frame.dataStack >= 1 with
+      | false -> 
+        let newDataStack = [undefinedBehavior "STORE_FAST"] in
+          execBytecode ({frame with dataStack = newDataStack; pc = frame.pc+1})
+      | true ->
+        let newLocalPlus, newDataStack = store_fast i (frame.f_localplus) 
+                                                      (frame.dataStack) in
+          execBytecode ({frame with dataStack = newDataStack;
+                                    pc = frame.pc+1;
+                                    f_localplus = newLocalPlus}))
+                                
     | MAKE_FUNCTION(flags) ->
-       let newDataStack = make_function flags (frame.f_globals) (frame.dataStack) in
+      (match length frame.dataStack >= 2 with
+      | false ->
+        let newDataStack = [undefinedBehavior "MAKE_FUNCTION"] in
+          execBytecode ({frame with dataStack = newDataStack; pc = frame.pc+1})
+      | true ->
+        let newDataStack = make_function flags (frame.f_globals)
+                                               (frame.dataStack) in
+          execBytecode ({frame with dataStack = newDataStack; pc = frame.pc+1}))
+    | _ -> 
+      let newDataStack = [undefinedBehavior "INSTRUCTION_NOT_SUPPORTED"] in
         execBytecode ({frame with dataStack = newDataStack; pc = frame.pc+1})
-   | _ -> All.failwith "Bytecode instruction is not implemented yet"
 
 (*
    - Runs the code in the frame and update the VM once it's done.
@@ -740,3 +1055,4 @@ let rec runFrame virM frame =
       } in
       let newVM: vm = {popVM with callStack = newCallerFrame::newCallStack} in
       runFrame newVM newCallerFrame
+
